# 高等数学预备知识

## 因式分解

$$
( a + b ) ^ { 3 } = a ^ { 3 } + 3 a ^ { 2 } b + 3 a b ^ { 2 } + b ^ { 3 }
$$

$$
( a - b ) ^ { 3 } = a ^ { 3 } - 3 a ^ { 2 } b + 3 a b ^ { 2 } - b ^ { 3 }
$$

$$
a ^ { 3 } - b ^ { 3 } = ( a - b ) ( a ^ { 2 } + a b + b ^ { 2 } )
$$

$$
a ^ { 3 } + b ^ { 3 } = ( a + b ) ( a ^ { 2 } - a b + b ^ { 2 } )
$$

### 二项式定理
$$
( x + y ) ^ { n } = \sum _ { k = 0 } ^ { n } C _ { n } ^ { k } x ^ { n - k } y ^ { k } = \left( \begin{array}  { l  }  { n } \\ { 0 } \end{array} \right) x ^ { n } y ^ { 0 } + \left( \begin{array}  { l  }  { n } \\ { 1 } \end{array} \right) x ^ { n - 1 } y ^ { 1 } + \left( \begin{array}  { l  }  { n } \\ { 2 } \end{array} \right) x ^ { n - 2 } y ^ { 2 } + \cdots + \left( \begin{array}  { l  }  { n } \\ { n - 1 } \end{array} \right) x ^ { 1 }
$$
